
### 4.1.1 Fermat定理 
若${f}(x)$在点$x_{0}$处取得极值，且$x_{0}$可导，则${f}'(x_{0})=0$
### 4.1.2 Rolle定理
（1）${f}(x)\in C[a,b]$\
（2）${f}(x)\in D(a,b)$\
（3）${f}(a)={f}(b)$\
$\Rightarrow \exists\xi \in (a,b),{f}' (\xi )=0$
### 4.1.3 Lagrange定理
（1）${f}(x)\in C[a,b]$\
（2）${f}(x)\in D(a,b)$\
$\Rightarrow \exists\xi \in (a,b),{f}' (\xi )=\frac{f(b)-f(a)}{b-a}$
#### Lagrange定理结论的另一种形式
$a<\xi<b \Rightarrow 0 < \frac{\xi-a}{b-a}<1,记\theta=\frac{\xi-a}{b-a}$\
$则\xi=a+\theta(b-a),从而定理的结论：\exists\theta\in(0,1),f(b)-f(a)={f}'[a+\theta(b-a)](b-a)$\
$若取a=x,b=x+\Delta x,则$\
$\exists\theta\in(0,1),{f}(x+\Delta x)-{f}(x)={f}'(x+\theta\Delta x)\Delta x$